src/simple-proof/proof/GeneralToTight.v
@@ -18,18 +18,18 @@ Require Import InvertibleTypes.
     This lemma corresponds to Lemma 3.5 in the paper.
 
     [inert G]                    #<br>#
-    [G @@ Sigma ⊢## x: {A: S..U}]        #<br>#
+    [G ⋆ Sigma ⊢## x: {A: S..U}]        #<br>#
     [――――――――――――――――――――――――――――]   #<br>#
-    [exists T. G @@ Sigma ⊢## x: {A: T..T}]   #<br>#
-    [G @@ Sigma ⊢# T <: U]               #<br>#
-    [G @@ Sigma ⊢# S <: T]                    *)
+    [exists T. G ⋆ Sigma ⊢## x: {A: T..T}]   #<br>#
+    [G ⋆ Sigma ⊢# T <: U]               #<br>#
+    [G ⋆ Sigma ⊢# S <: T]                    *)
 Lemma sel_premise: forall G Sigma x A U V,
   inert G ->
-  G @@ Sigma ⊢## x : typ_rcd (dec_typ A U V) ->
+  G ⋆ Sigma ⊢## x : typ_rcd (dec_typ A U V) ->
   exists T,
-    G @@ Sigma ⊢! trm_var (avar_f x) : typ_rcd (dec_typ A T T) /\
-    G @@ Sigma ⊢# T <: V /\
-    G @@ Sigma ⊢# U <: T.
+    G ⋆ Sigma ⊢! trm_var (avar_f x) : typ_rcd (dec_typ A T T) /\
+    G ⋆ Sigma ⊢# T <: V /\
+    G ⋆ Sigma ⊢# U <: T.
 Proof.
   introv HG Hinv.
   dependent induction Hinv.
@@ -44,15 +44,15 @@ Qed.
     This lemma corresponds to Lemma 3.4 in the paper.
 
     [inert G]              #<br>#
-    [G @@ Sigma ⊢# x: {A: S..U}]   #<br>#
+    [G ⋆ Sigma ⊢# x: {A: S..U}]   #<br>#
     [――――――――――――――――――――――]   #<br>#
-    [G @@ Sigma ⊢# x.A <: U]       #<br>#
-    [G @@ Sigma ⊢# S <: x.A]            *)
+    [G ⋆ Sigma ⊢# x.A <: U]       #<br>#
+    [G ⋆ Sigma ⊢# S <: x.A]            *)
 Lemma sel_replacement: forall G Sigma x A T U,
     inert G ->
-    G @@ Sigma ⊢# trm_var (avar_f x) : typ_rcd (dec_typ A T U) ->
-    (G @@ Sigma ⊢# typ_sel (avar_f x) A <: U /\
-     G @@ Sigma ⊢# T <: typ_sel (avar_f x) A).
+    G ⋆ Sigma ⊢# trm_var (avar_f x) : typ_rcd (dec_typ A T U) ->
+    (G ⋆ Sigma ⊢# typ_sel (avar_f x) A <: U /\
+     G ⋆ Sigma ⊢# T <: typ_sel (avar_f x) A).
 Proof.
   introv HG Hty.
   pose proof (tight_to_invertible HG Hty) as Hinv.
@@ -60,32 +60,32 @@ Proof.
   split; eauto using subtyp_trans_t, subtyp_sel1_t, subtyp_sel2_t.
 Qed.
 
-(** * General to Tight [⊢ to @@ Sigma ⊢#] *)
+(** * General to Tight [⊢ to ⋆ Sigma ⊢#] *)
 (** The following lemma corresponds to Theorem 3.3 in the paper.
     It says that in an inert environment, general typing ([ty_trm] [⊢]) can
     be reduced to tight typing ([ty_trm_t] [⊢#]).
     The proof is by mutual induction on the typing and subtyping judgements.
 
     [inert G]           #<br>#
-    [G @@ Sigma ⊢ t: T]          #<br>#
+    [G ⋆ Sigma ⊢ t: T]          #<br>#
     [――――――――――――――]    #<br>#
-    [G @@ Sigma ⊢# t: T] #<br># #<br>#
+    [G ⋆ Sigma ⊢# t: T] #<br># #<br>#
 
     and                 #<br># #<br>#
     [inert G]           #<br>#
-    [G @@ Sigma ⊢ S <: U]        #<br>#
+    [G ⋆ Sigma ⊢ S <: U]        #<br>#
     [――――――――――――――――]  #<br>#
-    [G @@ Sigma ⊢# S <: U]         *)
+    [G ⋆ Sigma ⊢# S <: U]         *)
 Lemma general_to_tight: forall G0,
   inert G0 ->
   (forall G Sigma t T,
-     G @@ Sigma ⊢ t : T ->
+     G ⋆ Sigma ⊢ t : T ->
      G = G0 ->
-     G @@ Sigma ⊢# t : T) /\
+     G ⋆ Sigma ⊢# t : T) /\
   (forall G Sigma T U,
-     G @@ Sigma ⊢ T <: U ->
+     G ⋆ Sigma ⊢ T <: U ->
      G = G0 ->
-     G @@ Sigma ⊢# T <: U).
+     G ⋆ Sigma ⊢# T <: U).
 Proof.
   intros G0 HG.
   apply ts_mutind; intros; subst; try solve [eapply sel_replacement; auto]; eauto.
@@ -94,8 +94,8 @@ Qed.
 (** The general-to-tight lemma, formulated for term typing. *)
 Lemma general_to_tight_typing: forall G Sigma t T,
   inert G ->
-  G @@ Sigma ⊢ t : T ->
-  G @@ Sigma ⊢# t : T.
+  G ⋆ Sigma ⊢ t : T ->
+  G ⋆ Sigma ⊢# t : T.
 Proof.
   intros. apply* general_to_tight.
 Qed.
