src/simple-proof/proof/Substitution.v
@@ -70,38 +70,38 @@ Ltac fold_subst :=
 
 (** The proof is by mutual induction on term typing, definition typing, and subtyping. *)
 Lemma subst_rules: forall y U,
-  (forall G Sigma t T, G @@ Sigma ⊢ t : T -> forall G1 G2 Sigma1 Sigma2 x,
+  (forall G Sigma t T, G ⋆ Sigma ⊢ t : T -> forall G1 G2 Sigma1 Sigma2 x,
     G = G1 & x ~ U & G2 ->
     ok (G1 & x ~ U & G2) ->
     x \notin fv_ctx_types G1 ->
     Sigma = Sigma1 & Sigma2 ->
     x \notin fv_sigma_types Sigma1 ->
-    G1 & (subst_ctx x y G2) @@ (Sigma1 & subst_sigma x y Sigma2) ⊢ trm_var (avar_f y) : subst_typ x y U ->
-    G1 & (subst_ctx x y G2) @@ (Sigma1 & subst_sigma x y Sigma2) ⊢ subst_trm x y t : subst_typ x y T) /\
-  (forall G Sigma d D, G @@ Sigma /- d : D -> forall G1 G2 Sigma1 Sigma2 x,
+    G1 & (subst_ctx x y G2) ⋆ (Sigma1 & subst_sigma x y Sigma2) ⊢ trm_var (avar_f y) : subst_typ x y U ->
+    G1 & (subst_ctx x y G2) ⋆ (Sigma1 & subst_sigma x y Sigma2) ⊢ subst_trm x y t : subst_typ x y T) /\
+  (forall G Sigma d D, G ⋆ Sigma /- d : D -> forall G1 G2 Sigma1 Sigma2 x,
     G = G1 & x ~ U & G2 ->
     ok (G1 & x ~ U & G2) ->
     x \notin fv_ctx_types G1 ->
     Sigma = Sigma1 & Sigma2 ->
     x \notin fv_sigma_types Sigma1 ->
-    G1 & (subst_ctx x y G2) @@ (Sigma1 & subst_sigma x y Sigma2) ⊢ trm_var (avar_f y) : subst_typ x y U ->
-    G1 & (subst_ctx x y G2) @@ (Sigma1 & subst_sigma x y Sigma2) /- subst_def x y d : subst_dec x y D) /\
-  (forall G Sigma ds T, G @@ Sigma /- ds :: T -> forall G1 G2 Sigma1 Sigma2 x,
+    G1 & (subst_ctx x y G2) ⋆ (Sigma1 & subst_sigma x y Sigma2) ⊢ trm_var (avar_f y) : subst_typ x y U ->
+    G1 & (subst_ctx x y G2) ⋆ (Sigma1 & subst_sigma x y Sigma2) /- subst_def x y d : subst_dec x y D) /\
+  (forall G Sigma ds T, G ⋆ Sigma /- ds :: T -> forall G1 G2 Sigma1 Sigma2 x,
     G = G1 & x ~ U & G2 ->
     ok (G1 & x ~ U & G2) ->
     x \notin fv_ctx_types G1 ->
     Sigma = Sigma1 & Sigma2 ->
     x \notin fv_sigma_types Sigma1 ->
-    G1 & (subst_ctx x y G2) @@ (Sigma1 & subst_sigma x y Sigma2) ⊢ trm_var (avar_f y) : subst_typ x y U ->
-    G1 & (subst_ctx x y G2) @@ (Sigma1 & subst_sigma x y Sigma2) /- subst_defs x y ds :: subst_typ x y T) /\
-  (forall G Sigma T V, G @@ Sigma ⊢ T <: V -> forall G1 G2 Sigma1 Sigma2 x,
+    G1 & (subst_ctx x y G2) ⋆ (Sigma1 & subst_sigma x y Sigma2) ⊢ trm_var (avar_f y) : subst_typ x y U ->
+    G1 & (subst_ctx x y G2) ⋆ (Sigma1 & subst_sigma x y Sigma2) /- subst_defs x y ds :: subst_typ x y T) /\
+  (forall G Sigma T V, G ⋆ Sigma ⊢ T <: V -> forall G1 G2 Sigma1 Sigma2 x,
     G = G1 & x ~ U & G2 ->
     ok (G1 & x ~ U & G2) ->
     x \notin fv_ctx_types G1 ->
     Sigma = Sigma1 & Sigma2 ->
     x \notin fv_sigma_types Sigma1 ->
-    G1 & (subst_ctx x y G2) @@ (Sigma1 & subst_sigma x y Sigma2) ⊢ trm_var (avar_f y) : subst_typ x y U ->
-    G1 & (subst_ctx x y G2) @@ (Sigma1 & subst_sigma x y Sigma2) ⊢ subst_typ x y T <: subst_typ x y V).
+    G1 & (subst_ctx x y G2) ⋆ (Sigma1 & subst_sigma x y Sigma2) ⊢ trm_var (avar_f y) : subst_typ x y U ->
+    G1 & (subst_ctx x y G2) ⋆ (Sigma1 & subst_sigma x y Sigma2) ⊢ subst_typ x y T <: subst_typ x y V).
 Proof.
   introv. apply rules_mutind; intros; subst; simpl;
             try (subst_solver || rewrite subst_open_commut_typ);
@@ -129,12 +129,12 @@ Qed.
 (** The substitution lemma for term typing.
     This lemma corresponds to Lemma 3.19 in the paper. *)
 Lemma subst_ty_trm: forall y U G Sigma x t T,
-    G & x ~ U @@ Sigma ⊢ t : T ->
+    G & x ~ U ⋆ Sigma ⊢ t : T ->
     ok (G & x ~ U) ->
     x \notin fv_ctx_types G ->
     x \notin fv_sigma_types Sigma ->
-    G @@ Sigma ⊢ trm_var (avar_f y) : subst_typ x y U ->
-    G @@ Sigma ⊢ subst_trm x y t : subst_typ x y T.
+    G ⋆ Sigma ⊢ trm_var (avar_f y) : subst_typ x y U ->
+    G ⋆ Sigma ⊢ subst_trm x y t : subst_typ x y T.
 Proof.
   intros.
   apply (proj51 (subst_rules y U)) with (G1:=G) (G2:=empty) (Sigma1:=Sigma) (Sigma2:=empty) (x:=x) in H;
@@ -143,12 +143,12 @@ Qed.
 
 (** The substitution lemma for definition typing. *)
 Lemma subst_ty_defs: forall y U G Sigma x ds T,
-    G & x ~ U @@ Sigma /- ds :: T ->
+    G & x ~ U ⋆ Sigma /- ds :: T ->
     ok (G & x ~ U) ->
     x \notin fv_ctx_types G ->
     x \notin fv_sigma_types Sigma ->
-    G @@ Sigma ⊢ trm_var (avar_f y) : subst_typ x y U ->
-    G @@ Sigma /- subst_defs x y ds :: subst_typ x y T.
+    G ⋆ Sigma ⊢ trm_var (avar_f y) : subst_typ x y U ->
+    G ⋆ Sigma /- subst_defs x y ds :: subst_typ x y T.
 Proof.
   intros.
   apply (proj53 (subst_rules y U)) with (G1:=G) (G2:=empty) (Sigma1:=Sigma) (Sigma2:=empty) (x:=x) in H;
@@ -168,9 +168,9 @@ Lemma renaming_def: forall G Sigma z T ds x,
     ok G ->
     z # G ->
     z \notin (fv_ctx_types G \u fv_sigma_types Sigma \u fv_defs ds \u fv_typ T) ->
-    G & z ~ open_typ z T @@ Sigma /- open_defs z ds :: open_typ z T ->
-    G @@ Sigma ⊢ trm_var (avar_f x) : open_typ x T ->
-    G @@ Sigma /- open_defs x ds :: open_typ x T.
+    G & z ~ open_typ z T ⋆ Sigma /- open_defs z ds :: open_typ z T ->
+    G ⋆ Sigma ⊢ trm_var (avar_f x) : open_typ x T ->
+    G ⋆ Sigma /- open_defs x ds :: open_typ x T.
 Proof.
   introv Hok Hnz Hnz' Hz Hx. rewrite subst_intro_typ with (x:=z). rewrite subst_intro_defs with (x:=z).
   eapply subst_ty_defs; auto. eapply Hz. rewrite <- subst_intro_typ. all: auto.
@@ -186,9 +186,9 @@ Lemma renaming_typ: forall G Sigma z T U t x,
     ok G ->
     z # G ->
     z \notin (fv_ctx_types G \u fv_sigma_types Sigma \u fv_typ U \u fv_typ T \u fv_trm t) ->
-    G & z ~ U @@ Sigma ⊢ open_trm z t : open_typ z T ->
-    G @@ Sigma ⊢ trm_var (avar_f x) : U ->
-    G @@ Sigma ⊢ open_trm x t : open_typ x T.
+    G & z ~ U ⋆ Sigma ⊢ open_trm z t : open_typ z T ->
+    G ⋆ Sigma ⊢ trm_var (avar_f x) : U ->
+    G ⋆ Sigma ⊢ open_trm x t : open_typ x T.
 Proof.
   introv Hok Hnz Hnz' Hz Hx. rewrite subst_intro_typ with (x:=z). rewrite subst_intro_trm with (x:=z).
   eapply subst_ty_trm; auto. eapply Hz. rewrite subst_fresh_typ. all: auto.
@@ -202,9 +202,9 @@ Qed.
     [G ⊢ t^x : T^x]         *)
 Lemma renaming_fresh : forall L G Sigma T u U x,
     ok G ->
-    (forall x : var, x \notin L -> G & x ~ T @@ Sigma ⊢ open_trm x u : U) ->
-    G @@ Sigma ⊢ trm_var (avar_f x) : T ->
-    G @@ Sigma ⊢ open_trm x u : U.
+    (forall x : var, x \notin L -> G & x ~ T ⋆ Sigma ⊢ open_trm x u : U) ->
+    G ⋆ Sigma ⊢ trm_var (avar_f x) : T ->
+    G ⋆ Sigma ⊢ open_trm x u : U.
 Proof.
   introv Hok Hu Hx. pick_fresh y.
   rewrite subst_intro_trm with (x:=y); auto.
